Translation to straightline code (first attempts, mostly working)

src/Experiments/SimplyTypedArithmetic.v
@@ -5529,11 +5529,12 @@ Module Compilers.
              | ident.Z_mul_split_concrete _ as idc
              | ident.Z.sub_get_borrow_concrete _ as idc
                => fun (x_y : _ * expr (_ * _) + (_ * expr _ + type.interp _) * (_ * expr _ + type.interp _))
-                  => match x_y return (_ * expr _ + (_ * expr _ + type.interp _) * (_ * expr _ + type.interp _)) with
+                  => let default _ := default_interp idc x_y in
+                     match x_y return (_ * expr _ + (_ * expr _ + type.interp _) * (_ * expr _ + type.interp _)) with
                      | inr (inr x, inr y) =>
                        let result := ident.interp idc (x, y) in
                        inr (inr (fst result), inr (snd result))
-                     | _ => default_interp idc x_y
+                     | _ => default tt
                      end
              | ident.Z.add_get_carry_concrete _ as idc
                => fun (x_y : _ * expr (_ * _) + (_ * expr _ + type.interp _) * (_ * expr _ + type.interp _))
@@ -7746,7 +7747,7 @@ Module X25519_32.
   Import PrintingNotations.
   Print base_25p5_carry_mul.
 (*
-base_25p5_carry_mul = 
+base_25p5_carry_mul =
 fun var : type -> Type =>
 (λ x : var (type.list (type.type_primitive type.Z) * type.list (type.type_primitive type.Z))%ctype,
  expr_let x0 := x₁ [[0]] *₆₄ x₂ [[0]] +₆₄
@@ -7885,7 +7886,7 @@ fun var : type -> Type =>
              type.list (type.type_primitive type.Z)))
 *)
 End X25519_32.
-*)
+ *)
 
 Module BarrettReduction.
   (* TODO : generalize to multi-word and operate on (list Z) instead of T; maybe stop taking ops as context variables *)
@@ -8618,7 +8619,7 @@ Module P192_64.
   Open Scope expr_scope.
   Set Printing Width 100000.
   Set Printing Depth 100000.
-  
+
   Local Notation "'mul64' '(' x ',' y ')'" :=
     (Z.cast2 (uint64, _)%core @@ (Z.mul_split_concrete 18446744073709551616 @@ (x , y)))%expr (at level 50) : expr_scope.
   Local Notation "'add64' '(' x ',' y ')'" :=
@@ -8627,7 +8628,7 @@ Module P192_64.
     (Z.cast2 (uint64, bool)%core @@ (Z.add_with_get_carry_concrete 18446744073709551616 @@ (c, x , y)))%expr (at level 50) : expr_scope.
   Local Notation "'adx64' '(' c ',' x ',' y ')'" :=
     (Z.cast bool @@ (Z.add_with_carry @@ (c, x , y)))%expr (at level 50) : expr_scope.
-  
+
   Print mulmod.
 (*
 mulmod = fun var : type -> Type => λ x : var (type.list (type.type_primitive type.Z) * type.list (type.type_primitive type.Z))%ctype,
@@ -8695,7 +8696,7 @@ Module P192_32.
     (Z.cast2 (uint32, bool)%core @@ (Z.add_get_carry_concrete 4294967296 @@ (x , y)))%expr (at level 50) : expr_scope.
   Local Notation "'adc32' '(' c ',' x ',' y ')'" :=
     (Z.cast2 (uint32, bool)%core @@ (Z.add_with_get_carry_concrete 4294967296 @@ (c, x , y)))%expr (at level 50) : expr_scope.
-  
+
   Print mulmod.
   (*
 mulmod = fun var : type -> Type => λ x : var (type.list (type.type_primitive type.Z) * type.list (type.type_primitive type.Z))%ctype,
@@ -8890,6 +8891,291 @@ Module P256_32.
 End P256_32.
 *)
 
+Require Import Coq.Program.Wf.
+
+Module Straightline.
+  Module expr.
+    Section with_var.
+      Context {var : type.type -> Type}.
+      Context {dummy_var : forall t, var t}.
+
+      Let uexpr t := @Uncurried.expr.expr ident.ident var t.
+
+      Inductive expr : type.type -> Type :=
+      | Scalar {t} : scalar t -> expr t
+      | LetInAppIdentZ {s d} : zrange -> ident.ident s (type.Z) -> scalar s -> (var (type.Z) -> expr d) -> expr d
+      | LetInAppIdentZZ {s d} : zrange * zrange -> ident.ident s (type.Z*type.Z) -> scalar s -> (var (type.Z*type.Z) -> expr d) -> expr d
+      with scalar : type.type -> Type :=
+           | Var t : var t -> scalar t
+           | TT : scalar (type.type_primitive type.unit)
+           | Pair {a b} : scalar a -> scalar b -> scalar (a * b)
+           | Cast : zrange -> scalar type.Z -> scalar type.Z
+           | Cast2 : zrange * zrange -> scalar (type.Z*type.Z) -> scalar (type.Z*type.Z)
+           | Fst {a b} : scalar (a * b) -> scalar a
+           | Snd {a b} : scalar (a * b) -> scalar b
+           | Primitive {t} : type.interp (type.type_primitive t) -> scalar t
+      .
+
+      Fixpoint dummy t : expr t := Scalar (Var t (dummy_var t)).
+
+      Definition scalar_of_uncurried_ident {s d} (idc : ident.ident s d)
+        : scalar s -> option (scalar d) :=
+        match idc in ident.ident s d return scalar s -> option (scalar d) with
+        | ident.Z.cast r => fun args => Some (Cast r args)
+        | ident.Z.cast2 r => fun args => Some (Cast2 r args)
+        | @ident.fst A B => fun args => Some (@Fst A B args)
+        | @ident.snd A B => fun args => Some (@Snd A B args)
+        | @ident.primitive p x => fun _ => Some (Primitive x)
+        | _ => fun _ => None
+        end.
+
+      Fixpoint scalar_of_uncurried {t} (e : uexpr t) : option (scalar t) :=
+          match e in Uncurried.expr.expr t return option (scalar t) with
+          | expr.Var t v as e => Some (Var t v)
+          | expr.TT as e => Some TT
+          | expr.Pair A B a b
+            => match scalar_of_uncurried a, scalar_of_uncurried b with
+               | Some x, Some y => Some (Pair x y)
+               | _, _ => None
+               end
+          | expr.AppIdent _ _ idc args
+            => match scalar_of_uncurried args with
+               | Some x => scalar_of_uncurried_ident idc x
+               | None => None
+               end
+          | _ => None
+          end.
+
+      Fixpoint range_type t : Type :=
+        match t with
+        | type.type_primitive type.Z => zrange
+        | type.prod x y => range_type x * range_type y
+        | _ => unit
+        end.
+
+      Definition invert_cast {t} (e : uexpr t)
+        : option (range_type t * uexpr t) :=
+        match invert_AppIdent e with
+        | Some (existT s (idc, x)) =>
+          (match idc in ident.ident s t return uexpr s -> option (range_type t * uexpr t) with
+           | ident.Z.cast r => fun x => Some (r, x)
+           | ident.Z.cast2 r => fun x => Some (r, x)
+           | _ => fun _ => None
+           end) x
+        | None => None
+        end.
+
+
+      (* if we have a cast, what we have is
+         cast r (AppIdent idc x')
+         where x' has type s and idc is s -> type.Z
+         and tx = type.Z
+
+         we want this to be translated to
+
+         (idc, x',
+       *)
+      (* ident.Let_In @@ (cast r x) => r, x *)
+      Definition invert_LetInCast {tx tC} (args : uexpr (tx * (tx -> tC)))
+        : option (range_type tx * uexpr tx * uexpr (tx -> tC)) :=
+        match invert_Pair args with
+        | Some (x, e) =>
+          match invert_cast x with
+          | Some (r, x') => Some (r, x', e)
+          | None => None
+          end
+        | None => None
+        end.
+
+
+      (* TODO : currently we look at the first application, which might be a cast. *)
+      Definition invert_LetInAppIdent {tx tC} (args : uexpr (tx * (tx -> tC)))
+        : option { s : type.type & (range_type tx * ident.ident s tx * scalar s * (var tx -> uexpr tC))%type } :=
+        match invert_LetInCast args with
+        | Some (r, x, e) =>
+          match invert_AppIdent x with
+          | Some (existT s idc_x') =>
+            match scalar_of_uncurried (snd idc_x') with
+            | Some x'' =>
+              match invert_Abs e with
+              | Some k => Some (existT _ s (r, fst idc_x', x'', k))
+              | None => None
+              end
+            | None => None
+            end
+          | None => None
+          end
+        | None => None
+        end.
+
+      Fixpoint depth {t} (e : uexpr t) : nat :=
+        match e with
+        | expr.Var _ _ => O
+        | expr.TT => O
+        | expr.AppIdent _ _ idc args => S (depth args)
+        | expr.App _ _ f x => S (Nat.max (depth f) (depth x))
+        | expr.Pair _ _ x y => S (Nat.max (depth x) (depth y))
+        | expr.Abs _ _ f => S (depth (f (dummy_var _)))
+        end.
+
+      Definition of_uncurried_step {t} (e : uexpr t)
+                 (of_uncurried : forall {t}, uexpr t -> expr t)
+                 : expr t :=
+        (match e in Uncurried.expr.expr t return expr t -> expr t with
+         | AppIdent s d idc args =>
+           (match idc in ident.ident s d return uexpr s -> expr d -> expr d with
+            | ident.Let_In tx tC =>
+              (fun args default =>
+                 match invert_LetInAppIdent args return expr tC with
+                 | Some (existT s (r, idc, x, k)) =>
+                   (match tx as tx0 return range_type tx0 -> ident.ident s tx0 -> (var tx0 -> expr tC) -> expr tC with
+                    | type.type_primitive type.Z =>
+                      fun r idc k => @LetInAppIdentZ s tC r idc x k
+                    | type.prod type.Z type.Z =>
+                      fun r idc k => @LetInAppIdentZZ s tC r idc x k
+                    | _ => fun _ _ _ => default
+                    end) r idc (fun y : var tx => of_uncurried (k y))
+                 | None => default
+                 end)
+            | _ => fun _ default => default
+            end) args
+         | _ as e =>
+           (fun default =>
+              match scalar_of_uncurried e with
+              | Some s => Scalar s
+              | None => default
+              end)
+         end) (dummy t).
+
+      (* TODO : uses fuel; ideally want a cleaner termination proof *)
+      Fixpoint of_uncurried (fuel : nat) {t} (e : uexpr t)
+        : expr t :=
+        match fuel with
+        | S fuel' => of_uncurried_step e (@of_uncurried fuel')
+        | O => dummy t
+        end.
+
+    End with_var.
+  End expr.
+
+  (* TODO : Can I avoid having dummy_var appear here? *)
+  Definition of_Expr {s d} (e : Expr (s->d)) (var : type -> Type) (x:var s) dummy_var : expr.expr d
+    :=
+      match invert_Abs (e var) with
+      | Some f => expr.of_uncurried (dummy_var:=dummy_var) (expr.depth (dummy_var:=dummy_var) (f x)) (f x)
+      | None => expr.dummy (dummy_var:=dummy_var) d
+      end.
+
+End Straightline.
+
+Module StraightlineTest.
+  Definition test : Expr (type.Z -> type.Z) :=
+    fun var =>
+      Abs
+        (fun (x : var type.Z) =>
+           AppIdent (var:=var) ident.Let_In
+               (Pair (AppIdent (var:=var) (ident.Z.cast r[0~>4294967295]%zrange) (AppIdent (var:=var) (ident.Z.shiftr 8) (Var x)))
+                     (Abs (fun x : var type.Z => expr.Var x)))).
+
+  Eval vm_compute in (Straightline.of_Expr test).
+
+  Definition test_mul : Expr (type.Z -> type.Z) :=
+    fun var =>
+      Abs
+        (fun (x : var type.Z) =>
+           AppIdent (var:=var) ident.Let_In
+               (Pair (AppIdent (var:=var) (ident.Z.cast r[0~>4294967295]%zrange) (AppIdent (var:=var) (ident.Z.shiftr 8) (Var x)))
+                     (Abs (fun x : var type.Z =>
+                             AppIdent ident.Let_In
+                                      (Pair (AppIdent (ident.Z.cast r[0~>4294967295]%zrange) (AppIdent ident.Z.mul (Pair (AppIdent (@ident.primitive type.Z 12) TT) (Var x))))
+                                            (Abs (fun x : var type.Z => Var x)))
+                             )))).
+  Eval vm_compute in (Straightline.of_Expr test_mul).
+End StraightlineTest.
+
+(*
+Module InlineOperations.
+  Section with_var.
+    Context {var : type.type -> Type} (op_match : forall t, @expr.expr ident.ident var t -> bool).
+
+    Fixpoint inline_op {t} (e : @expr.expr ident.ident var t) : @expr.expr ident.ident var t
+      :=
+        match e in expr.expr t return @expr.expr ident.ident var t with
+        | Var t _ as e => e
+        | TT as e
+          => e
+        | Pair A B a b
+          => Pair (@inline_op A a) (@inline_op B b)
+        | App s d f x => App (@inline_op _ f) (@inline_op _ x)
+        | Abs s d f => Abs (fun v => @inline_op _ (f v))
+        | AppIdent s d idc args
+          => inline_op_ident idc (@inline_op s args)
+        end.
+
+    (*
+       AppIdent ident.Let_In (Pair (AppIdent (ident.shiftr n) x) (Abs (fun y : var _ => F (Var _ y))))
+
+       =>
+
+       F (AppIdent (ident.shiftr n) x)
+     *)
+
+    Definition replace_num {t} (old : var type.Z) (new : @expr.expr ident.ident var type.Z) (e : @expr.expr ident.ident var t)
+      : @expr.expr ident.ident var t
+      := match e with
+         | Var _ v =>
+         | TT => TT
+                   |
+
+
+    Definition inline_if_match {tx tC} (args : @expr.expr ident.ident var (tx * (tx -> tC)))
+      : @expr.expr ident.ident var tC :=
+      let default _ := AppIdent (@ident.Let_In tx tC) args in
+      match invert_Pair args with
+      | Some (e, Abs s d k) =>
+        if op_match tx e then App k e else default tt
+      | None => default tt
+      end.
+
+    Definition inline_op_ident {s d} (idc : ident.ident s d)
+      : expr.expr s -> expr.expr d
+      :=
+        match idc in ident.ident s d return @expr.expr ident.ident var s -> expr.expr d with
+        | ident.Let_In tx tC => fun args : @expr.expr ident.ident var (tx * (tx -> tC)) =>
+                                  @inline_if_match tx tC args
+        | _ as i => fun args => AppIdent i args
+        end.
+
+    Fixpoint inline_op {t} (e : @expr.expr ident.ident var t) : @expr.expr ident.ident var t
+      :=
+        match e in expr.expr t return @expr.expr ident.ident var t with
+        | Var t _ as e => e
+        | TT as e
+          => e
+        | Pair A B a b
+          => Pair (@inline_op A a) (@inline_op B b)
+        | App s d f x => App (@inline_op _ f) (@inline_op _ x)
+        | Abs s d f => Abs (fun v => @inline_op _ (f v))
+        | AppIdent s d idc args
+          => inline_op_ident idc (@inline_op s args)
+        end.
+  End with_var.
+
+  Fixpoint shift_land_matcher {var} t (e : @expr.expr ident.ident var t) : bool :=
+    match e with
+    | AppIdent _ _ (ident.Z_cast _) args => shift_land_matcher _ args
+    | AppIdent _ _ (ident.Z_cast2 _) args => shift_land_matcher _ args
+    | AppIdent _ _ (ident.Z_land _) args => true
+    | AppIdent _ _ (ident.Z_shiftr _) args => true
+    | _ => false
+    end.
+
+  Definition inline_shiftr_and_land {t} (e : Expr t) : Expr t :=
+    fun var => inline_op shift_land_matcher (e _).
+
+End InlineOperations.
+*)
+
 Module MontgomeryReduction.
   Section MontRed'.
     Context (N R N' R' : Z).
@@ -8909,8 +9195,8 @@ Module MontgomeryReduction.
       dlet_nd t1_t2 := (BaseConversion.widemul Zlog2R n nout y N) in
       dlet_nd sum_carry := Rows.add (weight Zlog2R 1) 2 [fst lo_hi; snd lo_hi] t1_t2 in
       dlet_nd y' := Z.zselect (snd sum_carry) 0 N in
-      dlet_nd lo'' := fst (Z.sub_get_borrow_full R (nth_default 0 (fst sum_carry) 1) y') in
-      Z.add_modulo lo'' 0 N.
+      dlet_nd lo''_carry := Z.sub_get_borrow_full R (nth_default 0 (fst sum_carry) 1) y' in
+      Z.add_modulo (fst lo''_carry) 0 N.
 
     Local Lemma Hw : forall i, w i = R ^ Z.of_nat i.
     Proof.
@@ -9054,11 +9340,24 @@ Module Montgomery256.
          As montred256_correct.
   Proof. Time solve_rmontred machine_wordsize. Time Qed.
 
+  Import Straightline.expr.
   Import PrintingNotations.
-  Open Scope expr_scope.
-  Set Printing Width 100000.
-
+  Set Printing Depth 1000000.
+  Local Notation "'tZ'" := (type.type_primitive type.Z).
+  Eval lazy in (Straightline.of_Expr montred256).
+  (* TODO : why is the sub not cast when I remove fst? *)
   Print montred256.
+
+  (* Check bounds on the sub, make sure it's outputting Some *)
+  Locate interp.
+  Eval lazy in (ZRange.ident.option.interp (ident.Z.sub_get_borrow_concrete (2^256)) (Some uint256, Some uint256)).
+
+  Check ZRange.split_bounds.
+  Print ZRange.split_bounds.
+  (* TODO: apply the split_bounds updates from the barrett branch! That's what currently is fucking up *)
+
+(* TODO: to get the right kind of output operation, I probably want
+  to inline all these shifts/ands. *)
   (*
 montred256 = fun var : type -> Type => λ x : var (type.type_primitive type.Z * type.type_primitive type.Z)%ctype,
              expr_let x0 := (uint128)(x₁ >> 128) in
